

**Question 1:** (Section 2.4: #1a, #1b)

(a) There exists a rational number  $x$ , such that  $x^2 - 3x - 7 = 0$ . This statement is false, as the solutions to this polynomial are  $\frac{3}{2} \pm \frac{\sqrt{37}}{2}$ , and the square root of a non-square integer is irrational.

(b) There exists a real number  $x$ , such that  $x^2 + 1 = 0$ . This is false because the solutions to this polynomial are  $\pm i$ , which are imaginary.

**Question 2:** (Section 2.4: #2d, #2f)

(d) Consider  $m = 4$ . Then,  $\frac{m}{3} = \frac{4}{3} \notin \mathbb{Z}$ . The negation of the statement in English is 'there exists an integer  $m$  such that  $m$  divided by 3 is not an integer.'

(f) Consider  $x = \frac{\pi}{2}$ . Then,  $\tan^2 x + 1$  is undefined, and thus there can be no equality. The negation of the statement in English is that 'there exists a real number  $x$  such that the one more than the tangent squared of  $x$  is not equal to the secant squared of  $x$ .'

**Question 3:** (Section 2.4: #10a, #10b)

(a)  $[\forall x, y \in \mathbb{R}][ (x < y) \rightarrow (f(x) < f(y)) ]$ .

(b)  $[\exists x, y \in \mathbb{R}][ (x \geq y) \wedge f(x) < f(y) ]$ .

**Question 4:** (Section 3.2: #5)

*Proof.* We proceed by the contrapositive, which is the statement

If  $a$  and  $b$  are odd, then  $ab$  is odd.

Suppose that  $a$  and  $b$  are odd integers. So,  $a = 2k + 1, k \in \mathbb{Z}$  and  $b = 2l + 1, l \in \mathbb{Z}$ . Then  $ab = (2k + 1)(2l + 1) = 4lk + 2k + 2l + 1$ . Factoring, we get  $2(2lk + k + l) + 1$ , which is odd.  $\square$

**Question 5:** (Section 3.2: #10)

*Proof.* Suppose  $n$  is an arbitrary integer.

( $\rightarrow$ ) Suppose  $n$  is even. Then,  $n = 2k, k \in \mathbb{Z}$ . So,  $n^2 = 4k^2$ . Then,

$$n^2 \equiv 0 \pmod{4}.$$

Thus,  $4 \mid n^2$ .

( $\leftarrow$ ) We proceed by the contrapositive, which is the statement

If  $n$  is odd, then  $4 \nmid n^2$ .

Suppose  $n$  is odd. Then,  $n = 2k + 1, k \in \mathbb{Z}$ , and so  $n^2 = 4k^2 + 4k + 1$ . Factoring, we get  $n^2 = 4(k^2 + k) + 1$ . Thus,

$$n^2 \equiv 1 \pmod{4},$$

so  $4 \nmid n^2$ .

□

**Question 6:** (Section 3.3: #4)

*Proof.* We proceed via a proof by contradiction. Suppose that  $\exists r \in \mathbb{Q}$  such that  $r^3 = 2$ . Then,  $r$  can be expressed as  $\frac{a}{b}$  such that  $(a, b \in \mathbb{Z}), \gcd(a, b) = 1$ . Substituting in, we have  $\frac{a^3}{b^3} = 2$ . Rearranging, we get that

$$a^3 = 2b^3$$

By observation, we see that  $a^3$  is even.

**Lemma 1.** *If  $n^3$  is even, then  $n$  is even.*

*Proof.* We proceed via a proof by the contrapositive, which is the statement

If  $n$  is odd, then  $n^3$  is odd.

Suppose  $n$  is odd. Then,  $n = 2k + 1, k \in \mathbb{Z}$ . Expanding, we get  $n^3 = 8k^3 + 12k^2 + 6k + 1$ . Thus,  $n^3$  is odd. □

By Lemma 1, because  $a^3$  is even,  $a$  is also even. So, it can be written as  $a = 2k, k \in \mathbb{Z}$ . Plugging  $2k$  in for  $a$ , we find that  $8k^3 = 2b^3$ . So,

$$4k^3 = b^3.$$

By observation,  $b^3$  must also be even, and by Lemma 1,  $b$  must be even as well. So,  $a$  and  $b$  both have 2 as a factor; however, we stated previously that  $\gcd(a, b) = 1$ . Therefore, the assumption that  $r$  is a rational number leads to a contradiction, thus  $r$  must be irrational. □

**Question 7:** (a) *Proof.* From the definition of the biconditional, we have  $P \Leftrightarrow Q \equiv (P \rightarrow Q) \wedge (Q \rightarrow P)$ . Rewriting the implications in their logical form, we get

$$(P \leftarrow Q) \wedge (Q \rightarrow P) \equiv (\neg P \vee Q) \wedge (\neg Q \vee P).$$

Using the distributive properties of conjunctions and disjunctions, we find that

$$(\neg P \vee Q) \wedge (\neg Q \vee P) \equiv (\neg Q \wedge \neg P) \vee (\neg Q \wedge Q) \vee (\neg P \wedge P) \vee (P \wedge Q).$$

Eliminating the contradictions  $\neg P \wedge P$  and  $\neg Q \wedge Q$ , we obtain  $(\neg Q \wedge \neg P) \vee (P \wedge Q)$ . Thus,  $P \Leftrightarrow Q \equiv (P \wedge Q) \vee (\neg P \wedge \neg Q)$ . □

(b) *Proof.* Rewriting the LHS in terms of logical operators, we get

$$(P \rightarrow Q) \vee (P \rightarrow Q) \equiv (\neg P \vee Q) \vee (\neg P \vee R).$$

Using the associative properties of disjunctions, we can rewrite the expression into the form

$$(\neg P \vee Q) \vee (\neg P \vee R) \equiv (\neg P \vee \neg P) \vee (Q \vee R).$$

By idempotency, this is equivalent to  $\neg P \vee (Q \vee R)$ . This is the definition of an implication, so  $\neg P \vee (Q \vee R) \equiv P \rightarrow (Q \vee R)$ . Thus,  $(P \rightarrow Q) \vee (P \rightarrow R) \equiv P \rightarrow (Q \vee R)$ .  $\square$

**Question 8:** *Proof.* We proceed by contradiction. Suppose there exists  $x_0, y_0 \in \mathbb{Z}$  such that  $x_0^2 = 4y_0 + 3$ . We consider two cases.

Case 1:  $x_0$  is even. Then,  $x_0 = 2k, k \in \mathbb{Z}$ . Plugging into the original expression, we get  $4k^2 = 4y + 3$ . Taking the expression modulo 4, we get  $0 \equiv 3 \pmod{4}$ , which is a contradiction.

Case 2:  $x_0$  is not even. So,  $x_0$  is odd, and can be expressed as  $x_0 = 2k + 1, k \in \mathbb{Z}$ . Plugging into the original expression, we get  $4k^2 + 4k + 1 = 4y + 3$ . Taking the expression modulo 4, we get  $1 \equiv 3 \pmod{4}$ , which is a contradiction.

In both cases, we have contradictions, thus there cannot exist integer solutions  $x, y \in \mathbb{Z}$  such that  $x^2 = 4y + 3$ .  $\square$

**Question 9:** *Proof.* Suppose  $x, y \in \mathbb{R}$ , and  $0 < x < y$ . Because  $x$  and  $y$  are both non-zero,  $\frac{1}{xy}$  exists. We multiply the expression  $0 < x < y$  by  $\frac{1}{xy}$ , which preserves the order of the inequality by the multiplicativity axiom. This gives us

$$(0 < x < y)\left(\frac{1}{xy}\right) = 0 < \frac{1}{y} < \frac{1}{x}.$$

$\square$

**Question 10:** *Proof.* Suppose  $\epsilon \in \mathbb{R}$  and  $\epsilon > 0$ . Then, we know that  $\frac{1}{\epsilon} \in \mathbb{R}$  exists since  $\epsilon \neq 0$ . Because  $\frac{1}{\epsilon} \in \mathbb{R}$ , by the Archimedean Principle,  $\exists n \in \mathbb{Z}$  such that  $n > \frac{1}{\epsilon}$ . Because  $\epsilon > 0$ , we can say  $n \in \mathbb{Z}^+$ . By the transitivity axiom, because  $\frac{1}{\epsilon} > 0$  and  $n > \frac{1}{\epsilon}$ , we have the inequality

$$0 < \frac{1}{\epsilon} < n. \tag{1}$$

We showed in Problem 9 that if the inequality  $0 < x < y$  holds for some  $x, y \in \mathbb{R}$ , then  $0 < \frac{1}{y} < \frac{1}{x}$ . Applying that result to Equation (1), we know that  $0 < \frac{1}{n} < \epsilon$ . So,  $\frac{1}{n} < \epsilon$ . Thus, we are done.  $\square$